Improve `fresh_key_package`

fstar/new/MLS.fst
@@ -2,43 +2,45 @@ module MLS
 
 open MLS.Result
 
-// TODO: why?
-friend MLS.Crypto.Builtins
+#set-options "--fuel 0 --ifuel 0"
 
-let cs = {
-  MLS.Crypto.Builtins.kem_dh = Spec.Agile.DH.DH_Curve25519;
-  kem_hash = Spec.Hash.Definitions.SHA2_256;
-  aead = Spec.Agile.AEAD.CHACHA20_POLY1305;
-  kdf_hash = Spec.Hash.Definitions.SHA2_256;
-  signature = MLS.Crypto.Builtins.Ed_25519
-}
+let cs = Success?.v (MLS.Crypto.Derived.ciphersuite_from_nt MLS.NetworkTypes.CS_mls10_128_dhkemx25519_chacha20poly1305_sha256_ed25519)
 
 let group_id = MLS.TreeSync.Types.group_id_t
 let state g = s:MLS.TreeSync.Types.state_t { g == s.group_id }
 
-#set-options "--z3rlimit 100 --fuel 0 --ifuel 0"
 let fresh_key_package e { identity; signature_key } =
+  let open MLS.TreeSync.Types in
+  let open MLS.Crypto in
   let open MLS.NetworkTypes in
-  let version = PV_mls10 in
-  let cipher_suite = CS_mls10_128_dhkemx25519_chacha20poly1305_sha256_ed25519 in
-  let basic_credential = {
-    identity;
-    signature_scheme = SA_ed25519;
-    signature_key
+  let open MLS.NetworkBinder in
+  let open MLS.Parser in
+  let open MLS.Result in // Already opened, but we don't want Parser.bind in the scope
+  assume (hpke_private_key_length cs < 32);
+  key_pair <-- hpke_gen_keypair cs e;
+  let ((private_key: bytes), public_key) = key_pair in
+  let unsigned_leaf_package: leaf_package_t = {
+    credential = {
+      version = 0;
+      identity;
+      signature_key;
+    };
+    version = 0;
+    content = ps_leaf_package_content.serialize ({public_key});
+    extensions = (* TODO *) Seq.empty;
+    signature = Seq.empty;
   } in
-  let credential = C_basic basic_credential in
-  admit (); // TODO: don't know how to generate something sensible for extensions
-  let extensions = Seq.empty in
-  let signature = (* TODO *) Seq.empty in
-  MLS.Result.bind (MLS.Crypto.Builtins.hpke_gen_keypair cs e) (fun key_pair ->
-  let (private_key: bytes), public_key = key_pair in
-  let key_package: key_package_nt =
-    { public_key; cipher_suite; version; credential; extensions; signature }
-  in
-  let key_package: bytes = ps_key_package.MLS.Parser.serialize key_package in
-  MLS.Result.return (key_package, private_key))
+  signature <-- (
+    unsigned_key_package <-- treesync_to_keypackage cs unsigned_leaf_package;
+    let tbs = ps_key_package_tbs.serialize (key_package_get_tbs unsigned_key_package) in
+    assume (sign_nonce_length cs < 32);
+    sign_sign cs ( (* private signature key *) admit ()) tbs (mk_randomness (Seq.slice e 0 (sign_nonce_length cs)))
+  );
+  let leaf_package = { unsigned_leaf_package with signature } in
+  key_package <-- treesync_to_keypackage cs leaf_package;
+  return (ps_key_package.serialize key_package, private_key)
 
-#reset-options
+#push-options "--fuel 2"
 let create e { identity; signature_key } g =
   let c: MLS.TreeSync.Types.credential_t = {
     identity;
@@ -47,3 +49,12 @@ let create e { identity; signature_key } g =
   } in
   let t = MLS.TreeSync.create_tree 1 1 c (Seq.seq_of_list [ Some c ]) in
   MLS.TreeSync.Types.mk_initial_state g 1 1 t
+#pop-options
+
+
+let add #g state key_package = admit()
+let remove #g state p = admit()
+let update #g state e = admit()
+let send #g state e data = admit()
+let process_welcome_message w lookup = admit()
+let process_group_message #g state msg = admit()
