fstar/new/MLS.Crypto.Derived.fsti
@@ -6,7 +6,9 @@ open Lib.IntTypes
 open Lib.ByteSequence
 open MLS.NetworkTypes
 
-val ciphersuite_from_nt: cipher_suite_nt -> result ciphersuite
+val ciphersuite_from_nt: cs:cipher_suite_nt -> res:result ciphersuite{Success? res = normalize_term (List.mem cs [CS_mls10_128_dhkemx25519_aes128gcm_sha256_ed25519; CS_mls10_128_dhkemp256_aes128gcm_sha256_p256; CS_mls10_128_dhkemx25519_chacha20poly1305_sha256_ed25519])}
+
+
 val ciphersuite_to_nt: ciphersuite -> result cipher_suite_nt
 
 val expand_with_label: ciphersuite -> secret:bytes -> label:bytes -> context:bytes -> len:size_nat -> result (lbytes len)
